ClickMG.v
@@ -1,0 +1,337 @@
+Require Import Base.
+Require Import Circuit.
+Require Import StateSpace.
+Require Import Monad.
+
+Require Import List.
+Import ListNotations.
+Open Scope list_scope.
+
+Require Import MarkedGraph.
+Require Import Click.
+
+Import EnsembleNotation.
+Open Scope ensemble_scope.
+Require Import Coq.Program.Equality.
+
+Section ClickMG.
+  Variable name : Set.
+  Context `{eq_dec name}.
+
+Section TokenMG.
+
+  Inductive token_transition :=
+  | left_ack : token_transition
+  | left_req : token_transition
+  | right_req
+  | right_ack
+  | clk_rise
+  | clk_fall
+  .
+  Instance token_transition_eq_dec : eq_dec token_transition.
+  Proof.
+    constructor; intros x y;
+    destruct x; destruct y;
+      try (left; reflexivity); try (right; discriminate).
+  Defined.
+
+
+
+  Inductive stage_place : token_transition -> token_transition -> Set :=
+  (* L.ack -> L.req *)
+  (* CLK- -> L.req *)
+  (* R.req -> L.req *)
+  | left_ack_left_req : stage_place left_ack left_req
+  | clk_fall_left_req : stage_place clk_fall left_req
+  | right_req_left_req : stage_place right_req left_req
+
+  (* CLK+ -> L.ack *)
+  | clk_rise_left_ack : stage_place clk_rise left_ack
+  
+  (* CLK+ -> R.req *)
+  | clk_rise_right_req : stage_place clk_rise right_req
+
+  (* R.req -> R.ack *)
+  | right_req_right_ack : stage_place right_req right_req
+  
+  (* CLK- -> R.ack *)
+  (* L.ack -> R.ack *)
+  | clk_fall_right_ack : stage_place clk_fall right_ack
+  | left_ack_right_ack : stage_place left_ack right_ack
+  
+
+  (* CLK+ -> CLK- *)
+  | clock_fall : stage_place clk_rise clk_fall
+  
+  (* left_req -> CLK+ *)
+  (* right_ack -> CLK+ *)
+  | left_req_clk_rise : stage_place left_req clk_rise
+  | right_ack_clk_rise : stage_place right_ack clk_rise
+  .
+
+  Definition stage_MG : marked_graph token_transition :=
+    {| place := stage_place
+     ; init_marking := fun t1 t2 p => match p with
+                                      | left_req_clk_rise => 1
+                                      | right_ack_clk_rise => 1
+                                      | _ => 0
+                                      end
+     |}.
+
+  Variable even odd : Set.
+  Context `{naming_scheme name even odd}.
+  Variable dp_reset_n ctrl_reset_n : name.
+
+  Variable l : latch even odd.
+
+  Definition transition_update_value (t : token_transition) (v : value) : value :=
+    match t with
+    | clk_rise => Bit1
+    | clk_fall => Bit0
+    | _ => neg_value v
+    end.
+  Definition transition_name (t : token_transition) : name :=
+    match t with
+    | left_ack => ack (latch_input l)
+    | left_req => req (latch_input l)
+    | right_req => req (latch_output l)
+    | right_ack => ack (latch_output l)
+    | clk_rise  => latch_clk l
+    | clk_fall  => latch_clk l
+    end.
+    
+
+  Definition transition_to_event (t : token_transition) (σ : state name) : event name value :=
+    let x := transition_name t in
+    Event x (transition_update_value t (σ x)).
+(*
+    match t with
+    | left_ack => let n := (ack (latch_input l))
+                  in Event n (neg_value (σ n))
+    | left_req => let n := (req (latch_input l))
+                  in Event n (neg_value (σ n))
+    | right_req => let n := (req (latch_output l))
+                   in Event n (neg_value (σ n))
+    | right_ack => let n := (ack (latch_output l))
+                   in Event n (neg_value (σ n))
+    | clk_rise  => Event (latch_clk l) Bit1
+    | clk_fall  => Event (latch_clk l) Bit0
+    end.
+*)
+  Definition event_to_transition (e : event name value) : option token_transition :=
+    match e with
+    | Event x v => if x =? ack (latch_input l) then Some left_ack
+                   else if x =? req (latch_input l) then Some left_req
+                   else if x =? req (latch_output l) then Some right_req
+                   else if x =? ack (latch_output l) then Some right_ack
+                   else if x =? latch_clk l
+                        then if v =? Bit0 then Some clk_fall
+                             else if v =? Bit1 then Some clk_rise
+                             else None
+                   else None
+    end.
+
+
+  Definition visible_domain : list name :=
+       req (latch_input l) :: ack (latch_input l)
+    :: req (latch_output l) :: ack (latch_output l)
+    :: latch_clk l :: nil.
+  Hypothesis visible_disjoint : all_disjoint visible_domain.
+
+  Inductive event_equiv_transition_trace : tail_list (event name value) ->
+                                                 tail_list token_transition ->
+                                                 Prop :=
+  | equiv_t_empty : event_equiv_transition_trace t_empty t_empty
+(*
+  | equiv_left_ack t t' n v :
+    event_trace_equiv_transition_trace t t' ->
+    n = ack (latch_input l) ->
+    event_trace_equiv_transition_trace (t ▶ Event n v) (t' ▶ left_ack)
+  | equiv_left_req t t' n v :
+    event_trace_equiv_transition_trace t t' ->
+    n = req (latch_input l) ->
+    event_trace_equiv_transition_trace (t ▶ Event n v) (t' ▶ left_req)
+  | equiv_right_ack t t' n v :
+    event_trace_equiv_transition_trace t t' ->
+    n = ack (latch_output l) ->
+    event_trace_equiv_transition_trace (t ▶ Event n v) (t' ▶ right_ack)
+  | equiv_right_req t t' n v :
+    event_trace_equiv_transition_trace t t' ->
+    n = req (latch_output l) ->
+    event_trace_equiv_transition_trace (t ▶ Event n v) (t' ▶ right_req)
+  | equiv_clk_rise t t' n :
+    event_trace_equiv_transition_trace t t' ->
+    n = latch_clk l ->
+    event_trace_equiv_transition_trace (t ▶ Event n Bit1) (t' ▶ clk_rise)
+  | equiv_clk_fall t t' n v :
+    event_trace_equiv_transition_trace t t' ->
+    n = latch_clk l ->
+    event_trace_equiv_transition_trace (t ▶ Event n v) (t' ▶ clk_fall)
+*)
+  | equiv_t_cons t t' e e' :
+    event_equiv_transition_trace t t' ->
+    Some e' = event_to_transition e ->
+    event_equiv_transition_trace (t ▶ e) (t' ▶ e')
+
+  | equiv_event_hidden t t' x v :
+    event_equiv_transition_trace t t' ->
+    x ∉ from_list visible_domain ->
+    event_equiv_transition_trace (t ▶ Event x v) t'
+  .
+
+
+  Inductive state_equiv_marking : state name ->
+                                  tail_list (event name value) ->
+                                  marking stage_MG ->
+                                  tail_list token_transition ->
+                                  Prop :=
+  | state_equiv_marking0 (σ : state name) m : 
+    σ = σR l false ->
+    m = init_marking stage_MG ->
+    state_equiv_marking σ t_empty m t_empty
+
+  | state_equiv_marking_step σ σ' t t' (e : token_transition) (e' : event name value) m m':
+    state_equiv_marking σ t m t' ->
+    is_enabled stage_MG e m ->
+    e' = transition_to_event e σ ->
+    σ' = update_event σ e' ->
+    m' = fire e stage_MG m ->
+    state_equiv_marking σ' (t ▶ e') m' (t' ▶ e)
+
+  | state_equiv_marking_epsilon σ σ' t t' m :
+    state_equiv_marking σ t m t' ->
+    (forall n, n ∈ from_list visible_domain ->
+               σ n = σ' n) ->
+    state_equiv_marking σ' t m t'
+
+  | state_equiv_marking_internal σ t m t' σ' x v :
+    state_equiv_marking σ t m t' ->
+    σ' = update_event σ (Event x v) ->
+    x ∉ from_list visible_domain ->
+    state_equiv_marking σ' (t ▶ Event x v) m t'
+
+  .
+
+  Definition state_MG_traces : Ensemble (tail_list (event name value)) :=
+    fun t => exists σ m t', state_equiv_marking σ t m t'.
+
+  (* This is the hard lemma, I suspect *)
+  Lemma stage_implies_stage_MG_event : forall σ t m e σ' t',
+    state_equiv_marking σ t m t' ->
+    latch_stage l ⊢ σ →{Some (transition_to_event e σ)} Some σ' ->
+    is_enabled stage_MG e m.
+  Admitted.
+
+
+
+  Lemma transition_to_event_reverse : forall e σ,
+    event_to_transition (transition_to_event e σ) = Some e.
+  Proof.
+    intros e σ.
+    unfold visible_domain in visible_disjoint.
+    destruct e; simpl;
+      repeat (compare_next; try my_subst; try reflexivity; find_contradiction).
+  Qed.
+
+  Lemma event_equiv_transition_implies_state_equiv_marking : forall σ' t t' m,
+    latch_stage l ⊢ σR l false →*{t} Some σ' ->
+    [stage_MG]⊢ t' ↓ m ->
+    event_equiv_transition_trace t t' ->
+    state_equiv_marking σ' t m t'.
+  Proof.
+    intros σ' t t' m Hstep.
+    generalize dependent m. generalize dependent t'.
+
+    remember (latch_stage l) as S. 
+    generalize dependent HeqS.
+    remember (Some σ') as τ.
+    generalize dependent σ'.
+    induction Hstep; intros σ'' Heqτ HeqS; try inversion Heqτ; subst; try clear Heqτ;
+      intros t' m HMG Hequiv.
+    * inversion Hequiv; subst.
+      inversion HMG; subst.
+      constructor; auto.
+    * specialize (IHHstep _ eq_refl eq_refl).
+      inversion Hequiv; subst.
+      + inversion HMG; subst.
+        eapply state_equiv_marking_step; eauto.
+        { admit (* true *). }
+        { admit (* true, but harder to show *). }
+      + eapply state_equiv_marking_internal; auto.
+        { admit (* true, I think *). }
+    * specialize (IHHstep _ eq_refl eq_refl).
+      eapply state_equiv_marking_epsilon; eauto.
+      { admit (* true *). }
+  Admitted.
+
+Lemma event_to_transition_compose : forall x v e σ,
+    event_to_transition (Event x v) = Some e ->
+    v = transition_update_value e (σ (transition_name e)) ->
+    transition_to_event e σ = Event x v.
+Proof.
+    intros x v e σ He Hv.
+    unfold event_to_transition in He.
+    unfold transition_to_event.
+    repeat (compare_next; [inversion He; subst; auto | ]).
+    compare_next. 
+    compare_next.
+    { my_subst. reduce_eqb. inversion He; subst; auto. }
+    compare_next.
+    { my_subst. reduce_eqb. inversion He; subst; auto. }
+Qed.
+
+Lemma visible_domain_is_transition : forall x v,
+    x ∈ from_list visible_domain ->
+    exists e0, event_to_transition (Event x v) = Some e0.
+Admitted.
+
+Lemma transition_step_value : forall σ σ' x v e,
+    latch_stage l ⊢ σ →{Some (Event x v)} Some σ' ->
+    x ∈ from_list visible_domain ->
+    event_to_transition (Event x v) = Some e ->
+    v = transition_update_value e (σ (transition_name e)).
+Admitted.
+
+  Theorem stage_implies_stage_MG_traces : forall t σ',
+    latch_stage l ⊢ σR l false →*{t} Some σ' ->
+    exists m t', event_equiv_transition_trace t t' /\ ([stage_MG]⊢ t' ↓ m).
+  Proof.
+    intros t σ' Hstep.
+    remember (latch_stage l) as S.
+    remember (Some σ') as τ.
+    generalize dependent HeqS.
+    generalize dependent σ'.
+    induction Hstep; intros σ'' Heqτ HeqS; try inversion Heqτ; subst; try clear Heqτ.
+    * exists (init_marking stage_MG).
+      exists t_empty.
+      split; constructor.
+    * specialize (IHHstep _ eq_refl eq_refl).
+      destruct IHHstep as [m [t' [Hequiv HMG]]].
+      destruct e as [x v].
+
+      destruct (In_Dec (from_list visible_domain) x) as [Hin | Hnin].
+      + destruct (visible_domain_is_transition _ v Hin) as [e He].
+        assert (is_enabled stage_MG e m).
+        { eapply stage_implies_stage_MG_event.
+          { apply event_equiv_transition_implies_state_equiv_marking; eauto. }
+            
+          { erewrite event_to_transition_compose; eauto.
+            eapply transition_step_value; eauto.
+          }
+        }
+        exists (fire e stage_MG m).
+        exists (t' ▶ e).
+        split.
+        { constructor; auto.
+        }
+        { econstructor; eauto. }
+      + exists m. exists t'. split; auto.
+        apply equiv_event_hidden; auto.
+    * clear H2. specialize (IHHstep _ eq_refl eq_refl).
+      destruct IHHstep as [m [t' [Hequiv HMG]]].
+      exists m. exists t'. split; auto.
+  Qed.
+        
+
+  End TokenMG.
+End ClickMG.
